extraction/examples/MidlangCounterRefTypes.v
@@ -33,16 +33,16 @@ Instance MidlangBoxes : MidlangPrintConfig :=
      print_full_names := false |}.
 
 Definition midlang_translation_map :=
-  [(<%% @current_slot %%>, "current_slot");
-  (<%% @account_balance %%>, "account_balance");
-  (<%% @address_eqb %%>, "address_eq");
-  (<%% @ctx_amount %%>, "amount");
-  (<%% @ctx_from %%>, "from");
-  (<%% @Chain %%>, "ConCertChain");
-  (<%% @ContractCallContext %%>, "ConCertCallContext");
-  (<%% @ConCert.Execution.Blockchain.ActionBody %%>, "ConCertAction");
-  (<%% @ChainBase %%>, "ChainBaseWTF");
-  (<%% @ctx_contract_address %%>, "contract_address")].
+  [(<%%% @current_slot %%%>, "current_slot");
+  (<%%% @account_balance %%%>, "account_balance");
+  (<%%% @address_eqb %%%>, "address_eq");
+  (<%%% @ctx_amount %%%>, "amount");
+  (<%%% @ctx_from %%%>, "from");
+  (<%%% @Chain %%%>, "ConCertChain");
+  (<%%% @ContractCallContext %%%>, "ConCertCallContext");
+  (<%%% @ConCert.Execution.Blockchain.ActionBody %%%>, "ConCertAction");
+  (<%%% @ChainBase %%%>, "ChainBaseWTF");
+  (<%%% @ctx_contract_address %%%>, "contract_address")].
 
 Definition midlang_translate (name : kername) : option string :=
   match find (fun '(key, _) => eq_kername key name) midlang_translation_map with
@@ -111,16 +111,16 @@ Definition counter_name := <%% CounterRefinmentTypes.counter %%>.
 
 Definition TT : list (kername * string) := Eval compute in
   [
-       remap <%% Z.add %%> "add"
-     ; remap <%% Z.sub %%> "sub"
-     ; remap <%% Z.leb %%> "le"
-     ; remap <%% Z.ltb %%> "lt"
-     ; remap <%% Z %%> "Int"
-     ; ((<%% Z %%>.1, "Z0"),"0")
-     ; remap <%% nat %%> "AccountAddress"
-     ; remap <%% CounterRefinmentTypes.Transaction %%> "Transaction"
-     ; remap <%% CounterRefinmentTypes.Transaction_none %%> "Transaction.none"
-     ; remap <%% bool %%> "Bool" ].
+       remap <%%% Z.add %%%> "add"
+     ; remap <%%% Z.sub %%%> "sub"
+     ; remap <%%% Z.leb %%%> "le"
+     ; remap <%%% Z.ltb %%%> "lt"
+     ; remap <%%% Z %%%> "Int"
+     ; ((<%%% Z %%%>.1, "Z0"),"0")
+     ; remap <%%% nat %%%> "AccountAddress"
+     ; remap <%%% CounterRefinmentTypes.Transaction %%%> "Transaction"
+     ; remap <%%% CounterRefinmentTypes.Transaction_none %%%> "Transaction.none"
+     ; remap <%%% bool %%%> "Bool" ].
 
 Definition midlang_counter_translate (name : kername) : option string :=
   match find (fun '(key, _) => eq_kername key name) (TT ++ midlang_translation_map) with
@@ -130,13 +130,13 @@ Definition midlang_counter_translate (name : kername) : option string :=
 
 Definition ignored_concert_types :=
   Eval compute in
-        [<%% @ActionBody %%>;
-         <%% @Address %%>;
-         <%% @Amount %%>;
-         <%% @ChainBase %%>;
-         <%% @Chain %%>;
-         <%% @ContractCallContext %%>;
-         <%% @SerializedValue %%>].
+        [<%%% @ActionBody %%%>;
+         <%%% @Address %%%>;
+         <%%% @Amount %%%>;
+         <%%% @ChainBase %%%>;
+         <%%% @Chain %%%>;
+         <%%% @ContractCallContext %%%>;
+         <%%% @SerializedValue %%%>].
 
 
 Definition counter_extract :=
